ImpureAlarmConfig.v
@@ -1,0 +1,8 @@
+Require Import Vpl.Impure.
+Require Vpl.ImpureConfig.
+
+Module CoreAlarmed := AlarmImpureMonad Vpl.ImpureConfig.Core.
+Export CoreAlarmed.
+
+Ltac bind_imp_destruct H id1 id2 :=
+  apply CoreAlarmed.Base.mayReturn_bind in H; destruct H as [id1 [id2 H]].
