PolyLoop.v
@@ -1,0 +1,82 @@
+Require Import ZArith.
+Require Import List.
+Require Import Bool.
+Require Import Psatz.
+
+Require Import Linalg.
+Require Import Loop. (* for iter_semantics *)
+Require Import Misc.
+Require Import Instr.
+
+Open Scope Z_scope.
+
+Notation affine_expr := (positive * (list Z * Z))%type.
+Definition eval_affine_expr env (e : affine_expr) :=
+  (dot_product (fst (snd e)) (rev env) + snd (snd e)) / (Zpos (fst e)).
+Definition affine_expr_ok env (e : affine_expr) :=
+  ((dot_product (fst (snd e)) (rev env) + snd (snd e)) mod (Zpos (fst e)) =? 0).
+
+Inductive poly_stmt :=
+| PLoop : polyhedron -> poly_stmt -> poly_stmt
+| PInstr : instr -> list affine_expr -> poly_stmt
+| PSkip : poly_stmt
+| PSeq : poly_stmt -> poly_stmt -> poly_stmt
+| PGuard : polyhedron -> poly_stmt -> poly_stmt.
+
+Inductive poly_loop_semantics : poly_stmt -> list Z -> mem -> mem -> Prop :=
+| PLInstr : forall i es env mem1 mem2,
+(*    forallb (affine_expr_ok env) es = true -> *)
+    instr_semantics i (map (eval_affine_expr env) es) mem1 mem2 ->
+    poly_loop_semantics (PInstr i es) env mem1 mem2
+| PLSkip : forall env mem, poly_loop_semantics PSkip env mem mem
+| PLSeq : forall env st1 st2 mem1 mem2 mem3,
+    poly_loop_semantics st1 env mem1 mem2 ->
+    poly_loop_semantics st2 env mem2 mem3 ->
+    poly_loop_semantics (PSeq st1 st2) env mem1 mem3
+| PLGuardTrue : forall env t st mem1 mem2,
+    poly_loop_semantics st env mem1 mem2 ->
+    in_poly (rev env) t = true ->
+    poly_loop_semantics (PGuard t st) env mem1 mem2
+| PLGuardFalse : forall env t st mem,
+    in_poly (rev env) t = false -> poly_loop_semantics (PGuard t st) env mem mem
+| PLLoop : forall env p lb ub st mem1 mem2,
+    (forall x, in_poly (rev (x :: env)) p = true <-> lb <= x < ub) ->
+    iter_semantics (fun x => poly_loop_semantics st (x :: env)) (Zrange lb ub) mem1 mem2 ->
+    poly_loop_semantics (PLoop p st) env mem1 mem2.
+
+Lemma PLInstr_inv_sem :
+  forall i es env mem1 mem2,
+    poly_loop_semantics (PInstr i es) env mem1 mem2 ->
+    instr_semantics i (map (eval_affine_expr env) es) mem1 mem2.
+Proof.
+  intros i es env mem1 mem2 Hsem. inversion_clear Hsem. auto.
+Qed.
+
+Lemma PLLoop_inv_sem :
+  forall env p st mem1 mem2,
+    poly_loop_semantics (PLoop p st) env mem1 mem2 ->
+    exists lb ub, (forall x, in_poly (rev (x :: env)) p = true <-> lb <= x < ub) /\ iter_semantics (fun x => poly_loop_semantics st (x :: env)) (Zrange lb ub) mem1 mem2.
+Proof.
+  intros env p st mem1 mem2 H. inversion_clear H.
+  eexists; eexists; eauto.
+Qed.
+
+Lemma PLGuard_inv_sem :
+  forall env p st mem1 mem2,
+    poly_loop_semantics (PGuard p st) env mem1 mem2 ->
+    if in_poly (rev env) p then poly_loop_semantics st env mem1 mem2 else mem1 = mem2.
+Proof.
+  intros env p st mem1 mem2 H.
+  inversion_clear H.
+  - rewrite H1; simpl; auto.
+  - rewrite H0; simpl; auto.
+Qed.
+
+Lemma PLSeq_inv_sem :
+  forall env st1 st2 mem1 mem3,
+    poly_loop_semantics (PSeq st1 st2) env mem1 mem3 ->
+    exists mem2, poly_loop_semantics st1 env mem1 mem2 /\ poly_loop_semantics st2 env mem2 mem3.
+Proof.
+  intros env p st mem1 mem3 H.
+  inversion_clear H. exists mem2; auto.
+Qed.
